stash progress

src/base/adequacy.v
@@ -3,60 +3,79 @@ base logic. *)
 
 From iris.proofmode Require Import tactics.
 From iris.algebra Require Import auth.
-From Perennial.base_logic.lib Require Import proph_map.
-From Perennial.program_logic Require Import recovery_weakestpre recovery_adequacy.
-From Perennial.Helpers Require Import ipm.
+(* From Perennial.base_logic.lib Require Import proph_map. *)
+From self.program_logic Require Import recovery_weakestpre recovery_adequacy.
+(* From Perennial.Helpers Require Import ipm. *)
 
 From self Require Import ipm_tactics.
-From self.base Require Import cred_frag crash_borrow.
-From self.base Require Export wpr_lifting primitive_laws.
+(* From self.base Require Import cred_frag crash_borrow. *)
+From self.base Require Import wpr_lifting primitive_laws generational_resources.
+From self.nextgen Require Import nextgen_promises.
 
 Set Default Proof Using "Type".
 
-Definition nvm_build_base Σ (hpreG : nvmBaseGpreS Σ) (Hinv : invGS Σ) crIn
-           (cred_names : cr_names) : nvmBaseFixedG Σ :=
-  {|
-    nvmBaseG_invGS := Hinv;
-    nvmBaseG_gen_heapGS := nvmBase_preG_gen_heapGS;
-    nvmBaseG_crashGS := crIn;
-    view_inG := nvmBase_preG_view_inG;
-    crashed_at_inG := nvmBase_preG_crashed_at;
-    nvm_base_creditG :=
-      creditGS_update_pre Σ (nvmBase_preG_credit) cred_names;
-  |}.
+Definition nvm_build_base Σ (Ω : gGenCmras Σ): nvmBaseG Σ Ω.
+  refine (
+      {|
+        nvmBaseG_store_view_in := _;
+        store_view_name := _;
+        nvmBaseG_crashed_at_in := _;
+        crashed_at_name := _;
+        nvmBaseG_persisted_in := _;
+        persisted_name := _;
+        nvmBaseG_gmap_view_in := _;
+        heap_name := _;
+      |}).
+Admitted.
+
+(* Definition nvm_build_base Σ (hpreG : nvmBaseGpreS Σ) (Hinv : invGS Σ) crIn *)
+(*            (cred_names : cr_names) : nvmBaseFixedG Σ := *)
+(*   {| *)
+(*     nvmBaseG_invGS := Hinv; *)
+(*     nvmBaseG_gen_heapGS := nvmBase_preG_gen_heapGS; *)
+(*     nvmBaseG_crashGS := crIn; *)
+(*     view_inG := nvmBase_preG_view_inG; *)
+(*     crashed_at_inG := nvmBase_preG_crashed_at; *)
+(*     nvm_base_creditG := *)
+(*       creditGS_update_pre Σ (nvmBase_preG_credit) cred_names; *)
+(*   |}. *)
 
 (* Allocate the state intepretation in the base logic for any valid heap. *)
-Lemma allocate_state_interp `{hPre : !nvmBaseGpreS Σ} Hinv crIn γcrash σ PV cred_names :
+(* TODO: this lemma depends on the individual resource allocation lemmas in
+ * [base/generational_resources.v]. I need to finish those later. *)
+Lemma allocate_state_interp {Σ} {Ω: gGenCmras Σ}
+  (* `{hPre : !nvmBaseGpreS Σ} *)
+  Hinv Hcredit σ PV :
   valid_heap σ →
-  ⊢ |==> ∃ (hGD : nvmBaseDeltaG),
-    let hG := nvm_build_base _ hPre Hinv crIn cred_names in
-    ⌜ @crash_token_name hGD = γcrash ⌝ ∗
+  ⊢ |==>
+    let nvmG := nvm_build_base Σ Ω in
+    let PG := Build_PerennialG Σ Hinv Hcredit in
     nvm_heap_ctx (σ, PV) ∗
     ([∗ map] l↦v ∈ σ, l ↦h v) ∗
     validV ∅ ∗
     crashed_at ∅ ∗
     persisted PV.
 Proof.
-  intros val.
-  iMod (gen_heap_init_names σ) as (γh γm) "(yo & lo & holo)".
-  iMod (own_alloc (● max_view σ ⋅ ◯ ε)) as (store_view_name) "[HIP ?]".
-  { apply auth_both_valid_2; auto using view_valid, ucmra_unit_least. }
-  iMod (own_alloc (● PV ⋅ ◯ PV)) as (persist_view_name) "[? ?]".
-  { apply auth_both_valid_2; auto using view_valid. }
-  iMod (own_alloc (to_agree ∅ : agreeR viewO)) as (crashed_at_name) "#crashed".
-  { done. }
-  iExists ({| heap_names_name := {| name_gen_heap := γh; name_gen_meta := γm |};
-              crash_token_name := γcrash;
-              store_view_name := store_view_name;
-              persist_view_name := persist_view_name;
-              crashed_at_view_name := crashed_at_name |}).
-  iModIntro.
-  iFrame "∗#%".
-  rewrite /valid_heap.
-  rewrite /hist_inv.
-  iSplitPure; first done.
-  iExists _. iFrame "∗#". iPureIntro. rewrite dom_empty. set_solver.
-Qed.
+  (* intros val. *)
+  (* iMod (gen_heap_init_names σ) as (γh γm) "(yo & lo & holo)". *)
+  (* iMod (own_alloc (● max_view σ ⋅ ◯ ε)) as (store_view_name) "[HIP ?]". *)
+  (* { apply auth_both_valid_2; auto using view_valid, ucmra_unit_least. } *)
+  (* iMod (own_alloc (● PV ⋅ ◯ PV)) as (persist_view_name) "[? ?]". *)
+  (* { apply auth_both_valid_2; auto using view_valid. } *)
+  (* iMod (own_alloc (to_agree ∅ : agreeR viewO)) as (crashed_at_name) "#crashed". *)
+  (* { done. } *)
+  (* iExists ({| heap_names_name := {| name_gen_heap := γh; name_gen_meta := γm |}; *)
+  (*             crash_token_name := γcrash; *)
+  (*             store_view_name := store_view_name; *)
+  (*             persist_view_name := persist_view_name; *)
+  (*             crashed_at_view_name := crashed_at_name |}). *)
+  (* iModIntro. *)
+  (* iFrame "∗#%". *)
+  (* rewrite /valid_heap. *)
+  (* rewrite /hist_inv. *)
+  (* iSplitPure; first done. *)
+  (* iExists _. iFrame "∗#". iPureIntro. rewrite dom_empty. set_solver. *)
+Admitted.
 
 Section base_adequacy.
 
@@ -70,111 +89,113 @@ Section base_adequacy.
   [φinv] and [Φinv]). This makes the statement a bit more complex and we do not
   actually need the invariant feature at all. Hence we also have a simpler
   variant below for the case where the invariant is alwasy true.  *)
-  Theorem base_recv_adequacy Σ `{hPre : !nvmBaseGpreS Σ} s e r σ PV g φ φr φinv Φinv n :
+  Theorem base_recv_adequacy Σ (Ω: gGenCmras Σ) `{Hcredit: !cred_frag.creditGS Σ}
+    s e r σ PV g φ φr φinv Φinv :
     valid_heap σ →
-    (∀ `{Hheap : !nvmBaseFixedG Σ, hD : !nvmBaseDeltaG},
-      ⊢ pre_borrowN n -∗
+    (∀ `{!nvmBaseG Σ Ω} `{!PerennialG Σ},
+       ⊢
+        (* TODO: restore crash borrow after porting the dependencies *)
+        (* pre_borrowN n -∗ *)
         ([∗ map] l ↦ v ∈ σ, l ↦h v) -∗
         validV ∅ -∗
         persisted PV -∗ (
-          □ (∀ σ nt, state_interp σ nt -∗ |NC={⊤, ∅}=> ⌜ φinv σ ⌝) ∗
-          □ (∀ hGD, Φinv hGD -∗ □ ∀ σ nt, state_interp σ nt -∗ |NC={⊤, ∅}=> ⌜ φinv σ ⌝) ∗
-          wpr s ⊤ e r (λ v, ⌜φ v⌝) Φinv (λ _ v, ⌜φr v⌝))) →
+          (* TODO: confirm these modalities *)
+          ■ (∀ σ nt, state_interp σ nt -∗ |={⊤,∅}=> ⌜ φinv σ ⌝) ∗
+          ■ (Φinv -∗ □ ∀ σ nt, state_interp σ nt -∗ |={⊤,∅}=> ⌜ φinv σ ⌝) ∗
+          wpr s ⊤ e r (λ v, ⌜φ v⌝) Φinv (λ v, ⌜φr v⌝))) →
     recv_adequate (CS := nvm_crash_lang) s e r (σ, PV) g (λ v _ _, φ v) (λ v _ _, φr v) (λ σ _, φinv σ).
   Proof.
     intros val Hwp.
-    eapply (wp_recv_adequacy_inv _ _ _ _ _ _ _ _ _ _ _ _ _).
+    eapply (wp_recv_adequacy_inv _ _ _ _ _ _ _ _ _ _ _ _ _ _).
     (* eapply (wp_recv_adequacy_inv _ _ _ nvmBaseDeltaGO _ _ _ _ _ _ _ _ _ _). *)
-    iIntros (? [crIn γcrash] ?) "".
+    iIntros (? ?) "".
 
-    iMod (credit_name_init (n * 4 + crash_borrow_ginv_number)) as
-        (name_credit) "(Hcred_auth & Hcred & Htok)".
-    iDestruct (cred_frag_split with "Hcred") as "(Hpre & Hcred)".
-    iAssert (|={⊤}=> crash_borrow_ginv)%I with "[Hcred]" as ">#Hinv".
-    { rewrite /crash_borrow_ginv. iApply (inv_alloc _). iNext. eauto. }
+    (* iMod (credit_name_init (n * 4 + crash_borrow_ginv_number)) as *)
+    (*     (name_credit) "(Hcred_auth & Hcred & Htok)". *)
+    (* iDestruct (cred_frag_split with "Hcred") as "(Hpre & Hcred)". *)
+    (* iAssert (|={⊤}=> crash_borrow_ginv)%I with "[Hcred]" as ">#Hinv". *)
+    (* { rewrite /crash_borrow_ginv. iApply (inv_alloc _). iNext. eauto. } *)
 
-    set (crashPre := {| crash_inPreG := crIn |}).
-    iMod (allocate_state_interp Hinv crashPre γcrash σ PV name_credit)
-      as (hGD) "(%cEq & interp & pts & validV & crashedAt & pers)"; first done.
+    iMod (allocate_state_interp Hinv Hcredit σ PV)
+      as "(interp & pts & validV & crashedAt & pers)"; first done.
 
     (* Build an nvmBaseFixedG. *)
-    set (hG := nvm_build_base _ hPre Hinv crashPre name_credit).
+    set (nvmG := nvm_build_base Σ Ω).
+    set (PG := Build_PerennialG Σ Hinv Hcredit).
 
     iExists state_interp, global_state_interp, fork_post.
     iExists _, _.
-    iExists (
-      λ inv gen, ∃ nD', ⌜gen = nvmBase_generationGS (hGD := nD') ⌝ ∗ Φinv nD'
-    )%I.
+    iExists (λ inv, Φinv)%I.
 
-    iDestruct (@cred_frag_to_pre_borrowN _ hG _ _ n with "Hpre") as "Hpre".
-    iDestruct (Hwp hG hGD with "Hpre pts validV pers") as "(#H1 & #H2 & Hwp)".
+    (* iDestruct (@cred_frag_to_pre_borrowN _ hG _ _ n with "Hpre") as "Hpre". *)
+    iDestruct (Hwp nvmG PG with "pts validV pers") as "(#H1 & #H2 & Hwp)".
 
     iModIntro.
     iSplitR.
-    { iModIntro. simpl. rewrite cEq. iApply "H1". }
+    { iApply "H1". }
     iSplitR.
-    { iModIntro. iIntros (Hg') "(%nD' & -> & inv)".
-      iDestruct ("H2" with "inv") as "$". }
+    { iApply "H2". }
     iFrame.
-    iFrame "Hinv".
-    iSplit. { iPureIntro. done. }
-    rewrite /wpr.
-    rewrite /nvmBase_generationGS. rewrite cEq.
-    iApply (recovery_weakestpre.wpr_strong_mono with "Hwp").
-    iSplit; first by auto.
-    iSplit; first by auto.
-    by iIntros (??) "(% & _ & $)".
-  Qed.
+  Admitted.
+    (* iFrame "Hinv". *)
+    (* iSplit. { iPureIntro. done. } *)
+    (* rewrite /wpr. *)
+    (* rewrite /nvmBase_generationGS. rewrite cEq. *)
+    (* iApply (recovery_weakestpre.wpr_strong_mono with "Hwp"). *)
+    (* iSplit; first by auto. *)
+    (* iSplit; first by auto. *)
+    (* by iIntros (??) "(% & _ & $)". *)
+  (* Qed. *)
 
   (* Similar to the [recv_adequate] in Perennial except that:
     1. The invariant is removed.
     2. We ignore the global state (which is [unit] for nvm_lang). *)
-  Record recv_adequate (s : stuckness) (e1 r1 : thread_state) (σ1 : state nvm_lang)
-        (φ φr: thread_val → state nvm_lang → Prop) := {
-    recv_adequate_result_normal t2 σ2 v2 :
-      erased_rsteps (CS := nvm_crash_lang) r1 ([e1], (σ1, ())) (* NOTE: The unit is the unused global state. *)
-                    (thread_of_val v2 :: t2, (σ2, ())) Normal →
-      φ v2 σ2;
-    recv_adequate_result_crashed t2 σ2 v2 :
-      erased_rsteps (CS := nvm_crash_lang) r1 ([e1], (σ1, ()))
-                    (thread_of_val v2 :: t2, (σ2, ())) Crashed →
-      φr v2 σ2;
-    recv_adequate_not_stuck t2 σ2 e2 stat :
-      s = NotStuck →
-      erased_rsteps (CS := nvm_crash_lang) r1 ([e1], (σ1,())) (t2, (σ2,())) stat →
-      e2 ∈ t2 → (is_Some (thread_to_val e2) ∨ reducible (Λ := nvm_lang) e2 σ2 ());
-  }.
+  (* Record recv_adequate (s : stuckness) (e1 r1 : thread_state) (σ1 : state nvm_lang) *)
+  (*       (φ φr: thread_val → state nvm_lang → Prop) := { *)
+  (*   recv_adequate_result_normal t2 σ2 v2 : *)
+  (*     erased_rsteps (CS := nvm_crash_lang) r1 ([e1], (σ1, ())) (* NOTE: The unit is the unused global state. *) *)
+  (*                   (thread_of_val v2 :: t2, (σ2, ())) Normal → *)
+  (*     φ v2 σ2; *)
+  (*   recv_adequate_result_crashed t2 σ2 v2 : *)
+  (*     erased_rsteps (CS := nvm_crash_lang) r1 ([e1], (σ1, ())) *)
+  (*                   (thread_of_val v2 :: t2, (σ2, ())) Crashed → *)
+  (*     φr v2 σ2; *)
+  (*   recv_adequate_not_stuck t2 σ2 e2 stat : *)
+  (*     s = NotStuck → *)
+  (*     erased_rsteps (CS := nvm_crash_lang) r1 ([e1], (σ1,())) (t2, (σ2,())) stat → *)
+  (*     e2 ∈ t2 → (is_Some (thread_to_val e2) ∨ reducible (Λ := nvm_lang) e2 σ2 ()); *)
+  (* }. *)
 
-  Lemma adequacy_impl (s : stuckness) (e1 r1: thread_state) (σ1 : state nvm_lang)
-        (φ φr: thread_val → state nvm_lang → Prop) :
-    recovery_adequacy.recv_adequate (CS := nvm_crash_lang)
-                                    s e1 r1 σ1 () (λ v σ _, φ v σ) (λ v σ _, φr v σ) (λ _ _, True) →
-    recv_adequate s e1 r1 σ1 φ φr.
-  Proof. intros [????]. split; try naive_solver. Qed.
+  (* Lemma adequacy_impl (s : stuckness) (e1 r1: thread_state) (σ1 : state nvm_lang) *)
+  (*       (φ φr: thread_val → state nvm_lang → Prop) : *)
+  (*   recovery_adequacy.recv_adequate (CS := nvm_crash_lang) *)
+  (*                                   s e1 r1 σ1 () (λ v σ _, φ v σ) (λ v σ _, φr v σ) (λ _ _, True) → *)
+  (*   recv_adequate s e1 r1 σ1 φ φr. *)
+  (* Proof. intros [????]. split; try naive_solver. Qed. *)
 
-  (* This is the simpler adequacy result. *)
-  Corollary base_recv_adequacy_simpl Σ `{hPre : !nvmBaseGpreS Σ} s e r σ PV φ φr n :
-    valid_heap σ →
-    (∀ `{Hheap : !nvmBaseFixedG Σ, hD : !nvmBaseDeltaG},
-      ⊢ pre_borrowN n -∗
-        ([∗ map] l ↦ v ∈ σ, l ↦h v) -∗
-        persisted PV -∗
-        wpr s ⊤ e r (λ v, ⌜φ v⌝) (λ _, True) (λ _ v, ⌜φr v⌝)) →
-    recv_adequate s e r (σ, PV) (λ v _, φ v) (λ v _, φr v).
-  Proof.
-    intros val hyp.
-    apply adequacy_impl.
-    eapply (base_recv_adequacy Σ); first apply val.
-    intros nB nBD.
-    specialize (hyp nB nBD).
-    iIntros "borrow ptsMap crashedAt pers".
-    iDestruct (hyp with "borrow ptsMap pers") as "wpr".
-    iSplit.
-    { iIntros "!>" (? ?) "_". iApply ncfupd_mask_intro; naive_solver. }
-    iSplit.
-    { iIntros "!>" (?) "? !>". iIntros (? ?) "?".
-      iApply ncfupd_mask_intro; naive_solver. }
-    iFrame.
-  Qed.
+  (* (* This is the simpler adequacy result. *) *)
+  (* Corollary base_recv_adequacy_simpl Σ `{hPre : !nvmBaseGpreS Σ} s e r σ PV φ φr n : *)
+  (*   valid_heap σ → *)
+  (*   (∀ `{Hheap : !nvmBaseFixedG Σ, hD : !nvmBaseDeltaG}, *)
+  (*     ⊢ pre_borrowN n -∗ *)
+  (*       ([∗ map] l ↦ v ∈ σ, l ↦h v) -∗ *)
+  (*       persisted PV -∗ *)
+  (*       wpr s ⊤ e r (λ v, ⌜φ v⌝) (λ _, True) (λ _ v, ⌜φr v⌝)) → *)
+  (*   recv_adequate s e r (σ, PV) (λ v _, φ v) (λ v _, φr v). *)
+  (* Proof. *)
+  (*   intros val hyp. *)
+  (*   apply adequacy_impl. *)
+  (*   eapply (base_recv_adequacy Σ); first apply val. *)
+  (*   intros nB nBD. *)
+  (*   specialize (hyp nB nBD). *)
+  (*   iIntros "borrow ptsMap crashedAt pers". *)
+  (*   iDestruct (hyp with "borrow ptsMap pers") as "wpr". *)
+  (*   iSplit. *)
+  (*   { iIntros "!>" (? ?) "_". iApply ncfupd_mask_intro; naive_solver. } *)
+  (*   iSplit. *)
+  (*   { iIntros "!>" (?) "? !>". iIntros (? ?) "?". *)
+  (*     iApply ncfupd_mask_intro; naive_solver. } *)
+  (*   iFrame. *)
+  (* Qed. *)
 
 End base_adequacy.
