src/base/wpr_lifting.v
@@ -2,213 +2,208 @@ From stdpp Require Import numbers.
 From iris.proofmode Require Import tactics.
 From iris.algebra Require Import auth dfrac.
 (* From Perennial.base_logic.lib Require Import proph_map. *)
-From Perennial.program_logic Require Import recovery_weakestpre recovery_adequacy.
+(* From Perennial.program_logic Require Import recovery_weakestpre recovery_adequacy. *)
+From self.program_logic Require Import recovery_weakestpre recovery_adequacy.
 
 From self.nextgen Require Import omega.
 From self Require Import extra map_extra ipm_tactics if_non_zero view_slice.
 From self.lang Require Import lang.
-From self.base Require Import primitive_laws post_crash_modality.
+From self.base Require Import generational_resources primitive_laws.
+From self.nextgen Require Import nextgen_promises.
 
 Set Default Proof Using "Type".
 
-Definition wpr `{nvmBaseFixedG Σ, !extraStateInterp Σ, hG : nvmBaseDeltaG, Ω : gGenCmras Σ} `{hC : !crashGS Σ}
+Definition wpr `{!nvmBaseG Σ Ω, !extraStateInterp Σ, !PerennialG Σ}
            (s : stuckness) (E : coPset)
            (e : thread_state) (recv : thread_state) (Φ : thread_val → iProp Σ)
-           (Φinv : nvmBaseDeltaG → iProp Σ)
-           (Φr : nvmBaseDeltaG → thread_val → iProp Σ) :=
+           (Φinv : iProp Σ)
+           (Φr : thread_val → iProp Σ) :=
   wpr
-    nvm_crash_lang s _ E e recv Φ
-    (λ hGen, ∃ nvmD, ⌜hGen = nvmBase_generationGS (hGD := nvmD)⌝ ∗ Φinv nvmD)%I
-    (λ hGen v, ∃ nvmD, ⌜hGen = nvmBase_generationGS (hGD := nvmD)⌝ ∗ Φr nvmD v)%I.
+    nvm_crash_lang s E e recv Φ
+    (Φinv)%I
+    (λ v, Φr v)%I.
 
 Section wpr.
-  Context {Σ : gFunctors}.
+  Context {Σ : gFunctors} {Ω: gGenCmras Σ}.
   Implicit Types s : stuckness.
   Implicit Types P : iProp Σ.
   Implicit Types Φ : thread_val → iProp Σ.
-  Implicit Types Φc : nvmBaseDeltaG → iProp Σ.
+  Implicit Types Φc : iProp Σ.
   Implicit Types v : thread_val.
   Implicit Types e : thread_state.
 
-  Lemma wpr_strong_mono `{hG : !nvmBaseFixedG Σ, !extraStateInterp Σ, nvmBaseDeltaG, Ω : gGenCmras Σ}
+  Lemma wpr_strong_mono `{!nvmBaseG Σ Ω, !extraStateInterp Σ, !PerennialG Σ}
         s E e rec Φ Ψ Φinv Ψinv Φr Ψr :
     wpr s E e rec Φ Φinv Φr -∗
-    (∀ v, Φ v ==∗ Ψ v) ∧
-    ((∀ hG, Φinv hG -∗ Ψinv hG) ∧ (∀ hG v, Φr hG v ==∗ Ψr hG v)) -∗
+    (* TODO: what is this modality? *)
+    ■ ((∀ v, Φ v ==∗ Ψ v) ∧ ((Φinv -∗ Ψinv) ∧ (∀ v, Φr v ==∗ Ψr v))) -∗
     wpr s E e rec Ψ Ψinv Ψr.
   Proof.
     rewrite /wpr. iIntros "Hwpr Himpl".
     iApply (wpr_strong_mono with "Hwpr [Himpl]").
     repeat iSplit.
     - by iDestruct "Himpl" as "($ & _)".
-    - iIntros "% (% & % & ?)".
-      iDestruct "Himpl" as "(_ & H)".
-      iExists _. iSplit; first done. by iApply "H".
-    - iIntros "%% (% & % & ?)".
-      iDestruct "Himpl" as "(_ & H)".
-      iExists _. iSplitR; first done. by iApply "H".
+    - by iDestruct "Himpl" as "(_ & $ & _)".
+    - by iDestruct "Himpl" as "(_ & _ & $)".
   Qed.
 
-  Definition persist_auth `{nvmBaseFixedG, hGD : nvmBaseDeltaG}
-             (σ : mem_config) :=
-    own persist_view_name (● σ.2).
+  Definition persist_auth `{!nvmBaseG Σ Ω} (σ : mem_config): iProp Σ :=
+    ∃ OCV, persisted_auth (OCV `view_add` σ.2) ∗ crashed_at_offset OCV.
 
-  Lemma nvm_heap_reinit (hG : nvmBaseFixedG Σ) (hGD : nvmBaseDeltaG) σ PV CV
-        (γcrash : gname) :
-    (* The first two assumptions are the content of [crash_step σ σ'] *)
-    PV ⊑ CV →
-    consistent_cut CV σ →
-    valid_heap σ →
-    ⊢ gen_heap_interp (hG := _) σ -∗
-      persist_auth (σ, PV)
-      ==∗
-      ∃ (hGD' : nvmBaseDeltaG),
-        ⌜ @crash_token_name hGD' = γcrash ⌝ ∗
-        validV (hGD := hGD') ∅ ∗
-        post_crash_mapsto_map σ hGD hGD' ∗
-        nvm_heap_ctx (hGD := hGD') (slice_of_store CV σ, view_to_zero CV) ∗
-        persisted_impl hGD hGD' ∗
-        persisted (hGD := hGD') (view_to_zero CV) ∗
-        crashed_at (hGD := hGD') CV.
-  Proof using Σ.
-    iIntros (pIncl cut invs) "heapIntrp pers".
-    rewrite /nvm_heap_ctx. simpl.
-    (* Allocate a new heap at a _new_ ghost name. *)
-    iMod (gen_heap_init_names (slice_of_store CV σ)) as (γh γm) "(heapNew & ptsMap & _)".
-    (* We persist/freeze the old persist view. *)
-    iMod (own_update with "pers") as "pers".
-    { apply auth_update_auth_persist. }
-    iDestruct "pers" as "#oldPers".
-    (* Allocate a new persist view. *)
-    iMod (own_alloc (● (view_to_zero CV) ⋅ ◯ (view_to_zero CV))) as (persistG) "[pers #persFrag]".
-    { apply auth_both_valid_2; [apply view_valid|done]. }
-    (* Allocate the store view at a _new_ ghost name. *)
-    iMod (own_alloc (● max_view (slice_of_store CV σ) ⋅ ◯ ∅)) as (storeG) "[store fragStore]".
-    { apply auth_both_valid_2; [apply view_valid | apply: ucmra_unit_least]. }
-    (* Allocate the crashed at view at a _new_ ghost name. *)
-    iMod (own_alloc (to_agree CV : agreeR viewO)) as (crashedAtG) "#crashed".
-    { done. }
-    iModIntro.
-    set names := {| heap_names_name := Build_nvm_heap_names γh γm;
-                    crash_token_name := γcrash;
-                    store_view_name := storeG;
-                    persist_view_name := persistG;
-                    crashed_at_view_name := crashedAtG |}.
-    iExists names.
-    iSplitPure; first done.
-    rewrite /crashed_at_view_name. simpl.
-    iFrame.
-    iFrame "crashed persFrag".
-    (* We show the ghost crash relation. *)
-    iSplitL "ptsMap heapIntrp".
-    { rewrite /post_crash_mapsto_map.
-      iSplitL "heapIntrp".
-      { iIntros (???) "pts".
-        (* Set Printing All. *)
-        iApply (gen_heap_valid with "heapIntrp pts"). }
-      iDestruct (big_sepM_impl_strong _ _ _ σ with "ptsMap []") as "[$ _]".
-      iModIntro.
-      iIntros (ℓ hist) "pts". iIntros (look).
-      iApply soft_disj_intro_r.
-      iExists _. iFrame "crashed".
-      destruct (slice_of_store CV σ !! ℓ) as [?|] eqn:look'; last first.
-      * iRight. iPureIntro.
-        eapply consistent_cut_lookup_slice; done.
-      * iLeft.
-        rewrite /slice_of_store /slice_of_hist map_fmap_zip_with in look'.
-        rewrite map_fmap_zip_with in look'.
-        apply map_lookup_zip_with_Some in look'.
-        destruct look' as ([t] & ? & ? & CVLook & ?).
-        rewrite /consistent_cut in cut.
-        pose proof (map_Forall_lookup_1 _ _ _ _ cut CVLook) as (? & ? & ? & ? & map).
-        simplify_eq.
-        iExists _, _.
-        iSplit; first done.
-        rewrite H2.
-        rewrite map_fmap_singleton.
-        iFrame "pts".
-        iPureGoal; first done.
-        iPureIntro.
-        eapply (map_Forall_lookup_1 _ _ _ _ map).
-        rewrite /drop_above.
-        apply map_filter_lookup_Some_2; [done| reflexivity]. }
-    iSplit.
-    * simpl.
-      iSplit. { iPureIntro. apply store_inv_cut; done. }
-      iExists CV. iFrame "crashed".
-      (* TODO: Factor this out into a lemma (needs [cut] only). *)
-      apply consistent_cut_subseteq_dom in cut.
-      rewrite /slice_of_store /slice_of_hist map_fmap_zip_with.
-      rewrite map_fmap_zip_with.
-      rewrite dom_map_zip_with_eq_l; try done.
-    * iModIntro.
-      iIntros (V) "pers".
-      rewrite /persisted.
-      iDestruct (persisted_auth_included with "oldPers pers") as %incl.
-      assert (V ⊑ CV) as incl'. { etrans; done. }
-      iSplit.
-      { edestruct (view_to_zero_mono) as [? ->]; first apply incl'.
-        iDestruct "persFrag" as "[$ _]". }
-      iExists CV. iFrame "#%".
-  Qed.
+  (* Lemma nvm_heap_reinit σ PV CV `{!nvmBaseG} *)
+  (*       (γcrash : gname) : *)
+  (*   (* The first two assumptions are the content of [crash_step σ σ'] *) *)
+  (*   PV ⊑ CV → *)
+  (*   consistent_cut CV σ → *)
+  (*   valid_heap σ → *)
+  (*   ⊢ gen_heap_interp (hG := _) σ -∗ *)
+  (*     persist_auth (σ, PV) *)
+  (*     ==∗ *)
+  (*     ∃ (hGD' : nvmBaseDeltaG), *)
+  (*       ⌜ @crash_token_name hGD' = γcrash ⌝ ∗ *)
+  (*       validV (hGD := hGD') ∅ ∗ *)
+  (*       post_crash_mapsto_map σ hGD hGD' ∗ *)
+  (*       nvm_heap_ctx (hGD := hGD') (slice_of_store CV σ, view_to_zero CV) ∗ *)
+  (*       persisted_impl hGD hGD' ∗ *)
+  (*       persisted (hGD := hGD') (view_to_zero CV) ∗ *)
+  (*       crashed_at (hGD := hGD') CV. *)
+  (* Proof using Σ. *)
+  (*   iIntros (pIncl cut invs) "heapIntrp pers". *)
+  (*   rewrite /nvm_heap_ctx. simpl. *)
+  (*   (* Allocate a new heap at a _new_ ghost name. *) *)
+  (*   iMod (gen_heap_init_names (slice_of_store CV σ)) as (γh γm) "(heapNew & ptsMap & _)". *)
+  (*   (* We persist/freeze the old persist view. *) *)
+  (*   iMod (own_update with "pers") as "pers". *)
+  (*   { apply auth_update_auth_persist. } *)
+  (*   iDestruct "pers" as "#oldPers". *)
+  (*   (* Allocate a new persist view. *) *)
+  (*   iMod (own_alloc (● (view_to_zero CV) ⋅ ◯ (view_to_zero CV))) as (persistG) "[pers #persFrag]". *)
+  (*   { apply auth_both_valid_2; [apply view_valid|done]. } *)
+  (*   (* Allocate the store view at a _new_ ghost name. *) *)
+  (*   iMod (own_alloc (● max_view (slice_of_store CV σ) ⋅ ◯ ∅)) as (storeG) "[store fragStore]". *)
+  (*   { apply auth_both_valid_2; [apply view_valid | apply: ucmra_unit_least]. } *)
+  (*   (* Allocate the crashed at view at a _new_ ghost name. *) *)
+  (*   iMod (own_alloc (to_agree CV : agreeR viewO)) as (crashedAtG) "#crashed". *)
+  (*   { done. } *)
+  (*   iModIntro. *)
+  (*   set names := {| heap_names_name := Build_nvm_heap_names γh γm; *)
+  (*                   crash_token_name := γcrash; *)
+  (*                   store_view_name := storeG; *)
+  (*                   persist_view_name := persistG; *)
+  (*                   crashed_at_view_name := crashedAtG |}. *)
+  (*   iExists names. *)
+  (*   iSplitPure; first done. *)
+  (*   rewrite /crashed_at_view_name. simpl. *)
+  (*   iFrame. *)
+  (*   iFrame "crashed persFrag". *)
+  (*   (* We show the ghost crash relation. *) *)
+  (*   iSplitL "ptsMap heapIntrp". *)
+  (*   { rewrite /post_crash_mapsto_map. *)
+  (*     iSplitL "heapIntrp". *)
+  (*     { iIntros (???) "pts". *)
+  (*       (* Set Printing All. *) *)
+  (*       iApply (gen_heap_valid with "heapIntrp pts"). } *)
+  (*     iDestruct (big_sepM_impl_strong _ _ _ σ with "ptsMap []") as "[$ _]". *)
+  (*     iModIntro. *)
+  (*     iIntros (ℓ hist) "pts". iIntros (look). *)
+  (*     iApply soft_disj_intro_r. *)
+  (*     iExists _. iFrame "crashed". *)
+  (*     destruct (slice_of_store CV σ !! ℓ) as [?|] eqn:look'; last first. *)
+  (*     * iRight. iPureIntro. *)
+  (*       eapply consistent_cut_lookup_slice; done. *)
+  (*     * iLeft. *)
+  (*       rewrite /slice_of_store /slice_of_hist map_fmap_zip_with in look'. *)
+  (*       rewrite map_fmap_zip_with in look'. *)
+  (*       apply map_lookup_zip_with_Some in look'. *)
+  (*       destruct look' as ([t] & ? & ? & CVLook & ?). *)
+  (*       rewrite /consistent_cut in cut. *)
+  (*       pose proof (map_Forall_lookup_1 _ _ _ _ cut CVLook) as (? & ? & ? & ? & map). *)
+  (*       simplify_eq. *)
+  (*       iExists _, _. *)
+  (*       iSplit; first done. *)
+  (*       rewrite H2. *)
+  (*       rewrite map_fmap_singleton. *)
+  (*       iFrame "pts". *)
+  (*       iPureGoal; first done. *)
+  (*       iPureIntro. *)
+  (*       eapply (map_Forall_lookup_1 _ _ _ _ map). *)
+  (*       rewrite /drop_above. *)
+  (*       apply map_filter_lookup_Some_2; [done| reflexivity]. } *)
+  (*   iSplit. *)
+  (*   * simpl. *)
+  (*     iSplit. { iPureIntro. apply store_inv_cut; done. } *)
+  (*     iExists CV. iFrame "crashed". *)
+  (*     (* TODO: Factor this out into a lemma (needs [cut] only). *) *)
+  (*     apply consistent_cut_subseteq_dom in cut. *)
+  (*     rewrite /slice_of_store /slice_of_hist map_fmap_zip_with. *)
+  (*     rewrite map_fmap_zip_with. *)
+  (*     rewrite dom_map_zip_with_eq_l; try done. *)
+  (*   * iModIntro. *)
+  (*     iIntros (V) "pers". *)
+  (*     rewrite /persisted. *)
+  (*     iDestruct (persisted_auth_included with "oldPers pers") as %incl. *)
+  (*     assert (V ⊑ CV) as incl'. { etrans; done. } *)
+  (*     iSplit. *)
+  (*     { edestruct (view_to_zero_mono) as [? ->]; first apply incl'. *)
+  (*       iDestruct "persFrag" as "[$ _]". } *)
+  (*     iExists CV. iFrame "#%". *)
+  (* Qed. *)
 
-  Lemma nvm_heap_reinit_alt (hG : nvmBaseFixedG Σ) (hGD : nvmBaseDeltaG) σ σ'
-        (γcrash : gname) Pg :
-    crash_step σ σ' →
-    ⊢ nvm_heap_ctx σ -∗
-      post_crash Pg ==∗
-      ∃ names : nvmBaseDeltaG,
-        ⌜ @crash_token_name names = γcrash ⌝ ∗
-        post_crash_mapsto_map σ.1 hGD names ∗
-        nvm_heap_ctx (hGD := names) σ' ∗
-        Pg names.
+  (* Lemma nvm_heap_reinit_alt σ σ': *)
+  (*   crash_step σ σ' → *)
+  (*   ⊢ nvm_heap_ctx σ -∗ *)
+  (*      |==> ⚡==> |==> *)
+  (*       nvm_heap_ctx (hGD := names) σ' ∗ *)
+  (*       Pg names. *)
+  (* Proof. *)
+  (*   iIntros ([store p p' pIncl cut]). *)
+  (*   iIntros "(heap & authStor & %inv & pers & recov) Pg". *)
+  (*   iMod (nvm_heap_reinit _ _ _ _ _ γcrash with "heap pers") *)
+  (*     as (hGD') "(%crEq & _ & map & interp' & #persImpl & rec)"; try done. *)
+  (*   rewrite /post_crash. *)
+  (*   (* set newBundle : nvmBaseDeltaG := *) *)
+  (*   (*   {| nvmBaseDeltaG' := hnames |}. *) *)
+  (*   iSpecialize ("Pg" $! store hGD'). *)
+  (*   (* rewrite /newBundle. *) *)
+  (*   iDestruct ("Pg" with "persImpl map") as "(map & Pg)". *)
+  (*   iExists _. iModIntro. *)
+  (*   iSplitPure; first done. iFrame. *)
+  (* Qed. *)
+
+  (* Is this the only thing I need to prove for high spirea (other than views of course)? *)
+  Lemma extra_state_nextgen `{!nvmBaseG Σ Ω, !extraStateInterp Σ, !PerennialG Σ}:
+    extra_state_interp ⊢ |==> ⚡==> |==> extra_state_interp.
   Proof.
-    iIntros ([store p p' pIncl cut]).
-    iIntros "(heap & authStor & %inv & pers & recov) Pg".
-    iMod (nvm_heap_reinit _ _ _ _ _ γcrash with "heap pers")
-      as (hGD') "(%crEq & _ & map & interp' & #persImpl & rec)"; try done.
-    rewrite /post_crash.
-    (* set newBundle : nvmBaseDeltaG := *)
-    (*   {| nvmBaseDeltaG' := hnames |}. *)
-    iSpecialize ("Pg" $! store hGD').
-    (* rewrite /newBundle. *)
-    iDestruct ("Pg" with "persImpl map") as "(map & Pg)".
-    iExists _. iModIntro.
-    iSplitPure; first done. iFrame.
-  Qed.
+  Admitted.
 
-  Lemma idempotence_wpr `{nG : nvmBaseFixedG Σ, !extraStateInterp Σ, nD : nvmBaseDeltaG, Ω : gGenCmras Σ}
+  Lemma idempotence_wpr `{!nvmBaseG Σ Ω, !extraStateInterp Σ, !PerennialG Σ}
       s E1 e e_rec Φ Φinv Φr Φc :
-    ⊢ WPC e @ s; E1 {{ Φ }} {{ Φc nD }} -∗
-    (□ ∀ (nD1 : nvmBaseDeltaG),
-      Φc nD1 -∗ ▷ <PC> nD2, (Φinv nD2 ∧ WPC e_rec @ s ; E1 {{ Φr nD2 }} {{ Φc nD2 }})) -∗
+    ⊢ WPC e @ s; E1 {{ Φ }} {{ Φc }} -∗
+    (* TODO: have an expert double check this modality *)
+    ■ (Φc -∗ ▷ ⚡==> (Φinv ∧ WPC e_rec @ s ; E1 {{ Φr }} {{ Φc }})) -∗
       wpr s E1 e e_rec Φ Φinv Φr.
   Proof.
     iIntros "Hwpc #Hidemp".
-    iApply (
-      idempotence_wpr nvm_crash_lang s E1 e e_rec _ _ _
-                      (λ hGen, ∃ nvmD, ⌜hGen = nvmBase_generationGS (hGD := nvmD)⌝ ∗ Φc nvmD)%I
-                      with "[Hwpc] [Hidemp]"); first auto.
-    { iApply (wpc_crash_mono with "[] Hwpc").
-      iIntros "HΦcx". iExists _. destruct nG. by iFrame. }
-    { iModIntro. iIntros (HG' σ_pre_crash g σ_post_crash Hcrash ns mj D κs ?) "(%nvmD & %eq & phi)".
-      iMod (NC_alloc_strong) as (γcrash) "HNC".
-      iSpecialize ("Hidemp" $! _ with "phi").
-      rewrite eq.
-      iIntros "[interp extra] g !> !>".
-      iMod (nvm_heap_reinit_alt _ _ _ _ γcrash _ Hcrash with "interp Hidemp")
-        as (hnames) "(%cEq & map & interp' & idemp)".
-      set (hGD' := hnames).
-      iExists (nvmBase_generationGS (hGD := hGD')).
-      iMod (global_state_interp_le (Λ := nvm_lang) _ _ () _ _ κs with "[$]") as "$";
-        first (rewrite /step_count_next; simpl; lia).
+    iApply (idempotence_wpr nvm_crash_lang s E1 e e_rec _ _ _ Φc
+                            with "[$Hwpc] [Hidemp]").
+    (* { iApply (wpc_crash_mono with "[] Hwpc"). *)
+    (*   iIntros "HΦcx". iExists _. destruct nG. by iFrame. } *)
+    { iApply (plainly_mono with "[$]").
+      iIntros "Hidemp" (σ_pre_crash g σ_post_crash Hcrash ns mj D κs ?) "ϕc".
+      (* iMod (NC_alloc_strong) as (γcrash) "HNC". *)
+      iSpecialize ("Hidemp" with "ϕc").
+      (* rewrite eq. *)
+      iIntros "[interp extra] g".
+      (* iMod (nvm_heap_reinit_alt _ _ _ _ γcrash _ Hcrash with "interp Hidemp") *)
+      (*   as (hnames) "(%cEq & map & interp' & idemp)". *)
+      iMod (heap_ctx_next_generation _ _ Hcrash with "interp") as "interp".
+      iMod (extra_state_nextgen with "extra") as "extra".
+      do 3 iModIntro. iMod "interp". iMod "extra".
+      iAssert (global_state_interp g (step_count_next ns) mj D κs)%I as "$". { admit. }
+      (* iMod (global_state_interp_le (Λ := nvm_lang) _ _ () _ _ κs with "[$]") as "$"; *)
+      (*   first (rewrite /step_count_next; simpl; lia). *)
       iModIntro.
       rewrite /state_interp //=.
-      rewrite cEq.
       iFrame.
-      iSplit.
-      - iExists (hGD'). iDestruct "idemp" as "[$ _]". done.
-      - iDestruct "idemp" as "[_ H]". iApply (wpc_mono with "H"); eauto. }
-  Qed.
-
+  Admitted.
 End wpr.
